Proved the half part of serializability

src/Reduction.v
@@ -11,18 +11,6 @@ Ltac dest_step_m :=
          | [H: {| bst_oss := _ |} = {| bst_oss := _ |} |- _] => inv H
          end; simpl in *.
 
-Definition NonSilentHistory (hst: MHistory) :=
-  Forall (fun lbl => lbl <> RlblEmpty _) hst.
-
-Definition Internal (lbl: MLabel) :=
-  match lbl with
-  | RlblInt _ _ _ => True
-  | _ => False
-  end.
-
-Definition InternalHistory (hst: MHistory) :=
-  Forall (fun tlbl => Internal tlbl) hst.
-
 Definition Reduced (sys: System) (hfr hto: MHistory) :=
   forall st1 st2,
     steps step_m sys st1 hfr st2 ->
@@ -228,7 +216,7 @@ Qed.
 
 Lemma msg_ins_commutes_1:
   forall sys eins lbl,
-    Internal lbl ->
+    InternalLbl lbl ->
     Reduced sys [RlblIns eins; lbl] [lbl; RlblIns eins].
 Proof.
   unfold Reduced; intros.
@@ -332,7 +320,7 @@ Qed.
 
 Lemma msg_outs_commutes_1:
   forall sys eouts lbl,
-    Internal lbl ->
+    InternalLbl lbl ->
     Reduced sys [lbl; RlblOuts eouts] [RlblOuts eouts; lbl].
 Proof.
   unfold Reduced; intros.
