src/Denotation.v
@@ -1,0 +1,191 @@
+Require Import Bool List String Peano_dec.
+Require Import Common ListSupport FMap Syntax Semantics StepM StepT SemFacts.
+Require Import Topology Serial SerialFacts Reduction.
+
+Set Implicit Arguments.
+
+Definition Prec := MState -> Prop.
+Definition Trs := MState -> MState.
+
+Definition DenotationalL (sys: System) (prec: Prec) (trs: Trs) (hst: MHistory) :=
+  forall st1,
+    prec st1 ->
+    steps step_m sys st1 hst (trs st1).
+
+Definition DenotationalR (sys: System) (prec: Prec) (trs: Trs) (hst: MHistory) :=
+  forall st1 st2,
+    steps step_m sys st1 hst st2 ->
+    prec st1 /\ st2 = trs st1.
+
+Definition Denotational (sys: System) (prec: Prec) (trs: Trs) (hst: MHistory) :=
+  DenotationalL sys prec trs hst /\
+  DenotationalR sys prec trs hst.
+
+Definition NonconflictingD (p1 p2: Prec) (f1 f2: Trs) :=
+  (forall o, p2 (f1 o) -> p2 o) /\
+  (forall o, p1 o -> p1 (f2 o)) /\
+  (forall o, f2 (f1 o) = f1 (f2 o)).
+
+Lemma silent_denotational:
+  forall sys, Denotational sys (fun _ => True) id [RlblEmpty _].
+Proof.
+  intros.
+  hnf; split; hnf; intros.
+  - repeat econstructor.
+  - inv H; inv H3; inv H5; auto.
+Qed.
+
+Lemma ins_denotational:
+  forall sys eins,
+    eins <> nil ->
+    ValidMsgsExtIn sys eins ->
+    Denotational sys (fun _ => True)
+                 (fun st => {| bst_oss := bst_oss st;
+                               bst_orqs := bst_orqs st;
+                               bst_msgs := enqMsgs eins (bst_msgs st) |})
+                 [RlblIns eins].
+Proof.
+  intros.
+  hnf; split; hnf; intros.
+  - econstructor.
+    + econstructor.
+    + econstructor; eauto.
+      destruct st1; reflexivity.
+  - inv H1; inv H5; inv H7; auto.
+Qed.
+
+Lemma outs_denotational:
+  forall sys eouts,
+    eouts <> nil ->
+    ValidMsgsExtOut sys eouts ->
+    Denotational sys (fun st => Forall (FirstMPI (bst_msgs st)) eouts)
+                 (fun st => {| bst_oss := bst_oss st;
+                               bst_orqs := bst_orqs st;
+                               bst_msgs := deqMsgs (idsOf eouts) (bst_msgs st) |})
+                 [RlblOuts eouts].
+Proof.
+  intros.
+  hnf; split; hnf; intros.
+  - econstructor.
+    + econstructor.
+    + econstructor; eauto.
+      destruct st1; reflexivity.
+  - inv H1; inv H5; inv H7; auto.
+Qed.
+
+Inductive DenoteIntHst: Prec -> Trs -> MHistory -> Prop :=
+| DenoteNil: DenoteIntHst (fun _ => True) id nil
+| DenoteCons:
+    forall p f hst,
+      DenoteIntHst p f hst ->
+      forall rule ins outs,
+        DenoteIntHst
+          (fun st =>
+             p st /\
+             let oss := bst_oss (f st) in
+             let orqs := bst_orqs (f st) in
+             let msgs := bst_msgs (f st) in
+             Forall (FirstMPI msgs) ins /\
+             exists ost orq,
+               oss@[rule_oidx rule] = Some ost /\
+               orqs@[rule_oidx rule] = Some orq /\
+               rule_precond rule ost orq ins /\
+               snd (rule_trs rule ost orq ins) = outs
+          )
+          (fun st =>
+             let oss := bst_oss (f st) in
+             let orqs := bst_orqs (f st) in
+             let msgs := bst_msgs (f st) in
+             oss@[rule_oidx rule] >>=[st]
+                (fun ost =>
+                   orqs@[rule_oidx rule] >>=[st]
+                       (fun orq =>
+                          match rule_trs rule ost orq ins with
+                          | (nost, norq, _) =>
+                            {| bst_oss := oss +[rule_oidx rule <- nost];
+                               bst_orqs := orqs +[rule_oidx rule <- norq];
+                               bst_msgs := enqMsgs outs (deqMsgs (idsOf ins) msgs)
+                            |}
+                          end)))
+          (RlblInt rule ins outs :: hst).
+
+Lemma denoteIntHst_prec_trs_exist:
+  forall hst,
+    InternalHistory hst ->
+    exists p f, DenoteIntHst p f hst.
+Proof.
+  induction hst; simpl; intros.
+  - do 2 eexists; constructor.
+  - inv H.
+    specialize (IHhst H3).
+    destruct IHhst as [pp [pf ?]].
+    destruct a as [| |rule ins outs|]; try (elim H2; fail).
+    do 2 eexists.
+    econstructor; eauto.
+Qed.
+
+Lemma denoteIntHst_denotationalL:
+  forall sys p f hst,
+    WfHistory sys hst ->
+    DenoteIntHst p f hst ->
+    DenotationalL sys p f hst.
+Proof.
+  induction 2; simpl; intros; [constructor|].
+  inv H; econstructor; [destruct H; eapply IHDenoteIntHst; eauto|].
+  dest.
+  remember (rule_trs rule x x0 ins) as nst.
+  destruct nst as [[noss norqs] nmsgs].
+  apply eq_sym in Heqnst.
+  simpl in H7; subst.
+  red in H3; dest.
+  econstructor; try reflexivity; try eassumption; simpl.
+  - destruct (f st1); reflexivity.
+  - rewrite H2, H5; simpl.
+    rewrite Heqnst; reflexivity.
+Qed.
+
+Lemma denoteIntHst_denotationalR:
+  forall sys p f hst,
+    DenoteIntHst p f hst ->
+    DenotationalR sys p f hst.
+Proof.
+  induction 1; simpl; intros;
+    [red; intros; inv H; auto|].
+
+  red; intros; inv H0.
+  specialize (IHDenoteIntHst _ _ H4); dest; subst.
+  inv H6; rewrite H21; simpl.
+  repeat split; auto.
+  - do 2 eexists; repeat split; try eassumption.
+    rewrite H16; reflexivity.
+  - rewrite H8, H9; simpl.
+    rewrite H16; reflexivity.
+Qed.
+
+Lemma denoteIntHst_denotational:
+  forall sys p f hst,
+    WfHistory sys hst ->
+    DenoteIntHst p f hst ->
+    Denotational sys p f hst.
+Proof.
+  intros; split.
+  - apply denoteIntHst_denotationalL; auto.
+  - apply denoteIntHst_denotationalR; auto.
+Qed.
+
+Lemma atomic_denotational:
+  forall sys inits ins hst outs eouts,
+    WfHistory sys hst ->
+    Atomic msg_dec inits ins hst outs eouts ->
+    exists p f,
+      Denotational sys p f hst /\
+      DenoteIntHst p f hst.
+Proof.
+  intros.
+  apply atomic_internal_history in H0.
+  apply denoteIntHst_prec_trs_exist in H0.
+  destruct H0 as [p [f ?]].
+  pose proof (denoteIntHst_denotational H H0).
+  eauto.
+Qed.
+
